hw3/hw3-ord.thy
@@ -1,0 +1,36 @@
+theory "hw3-ord" 
+imports ZF 
+begin
+
+(* Lemma 8 *) 
+lemma transset_union : 
+  "Transset(i) \<Longrightarrow> 
+   Transset(j) \<Longrightarrow> 
+   Transset(i \<union> j)"
+  unfolding Transset_def
+  apply clarify 
+  by blast
+
+lemma ord_union : 
+  "Ord(i) \<Longrightarrow> 
+   Ord(j) \<Longrightarrow> 
+   Ord(i \<union> j)"
+  unfolding Ord_def
+  apply clarify 
+  using transset_union by blast
+
+(* Note induction on the number of ordinals in A doesn't make sense *)
+lemma transset_Union : 
+  "\<forall> i \<in> A . Transset(i) \<Longrightarrow> 
+   Transset (\<Union> A)"
+  unfolding Transset_def 
+  apply clarify 
+  by blast
+
+theorem ord_Union : 
+  "\<forall> i \<in> A . Ord(i) \<Longrightarrow> 
+   Ord (\<Union> A)"
+  unfolding Ord_def 
+  using transset_Union by blast
+
+end
